<?xml version="1.0" encoding="utf-8"?>
<!DOCTYPE rdf:RDF>

<rdf:RDF xmlns:rdf="http://www.w3.org/1999/02/22-rdf-syntax-ns#"
    xmlns:rdfs="http://www.w3.org/2000/01/rdf-schema#"
    xmlns:dc="http://dublincore.org/2012/06/14/dcelements.rdf#"
    xmlns:dct="http://dublincore.org/2012/06/14/dcterms.rdf#" 
    xmlns:aps="http://jacobshelby.org/schemas/aps/2014/08/03/apsSchema.rdf#"
    xml:base="http://jacobshelby.org/schemas/aps/2014/08/03/apsSchema.rdf#"
    xmlns:jes="http://slis.indiana.edu/~ejacob/jes-2013-fall/2013-10-23.rdf#">

    <rdf:Description rdf:about="http://jacobshelby.org/schemas/aps/2014/08/03/apsSchema.rdf">
        <dc:title>Audio Preservation Schema</dc:title>
        <dc:creator>Jacob Shelby</dc:creator>
        <dc:description>The Audio Preservation Schema element set is a set of metadata elements
            (classes and properties) designed to supply critical preservation information about a
            sound recording in order to further preserve and carefully digitize the sound recording.
            The elements in this schema are largely based on FACET: Format Characteristics and Preservation Problems, written by
            Michael Casey.</dc:description>
        <jes:dateCreated>2013-11-17</jes:dateCreated>
        <dct:created>2013-11-17</dct:created>
        <jes:dateLastModified>2014-08-03</jes:dateLastModified>
    </rdf:Description>

    <rdf:Property rdf:ID="bitDepth">
        <rdfs:label xml:lang="en">bit depth</rdfs:label>
        <rdfs:comment>Indicates the number of bits of information per sample, measured in bits, used
            to record the sound recording (ex. 16 bit)</rdfs:comment>
    </rdf:Property>

    <rdf:Property rdf:ID="brand">
        <rdfs:label xml:lang="en">brand</rdfs:label>
        <rdfs:comment>Acts as a wrapper for information about the brand of the
            carrier</rdfs:comment>
    </rdf:Property>

    <rdf:Property rdf:ID="brandName">
        <rdfs:label xml:lang="en">brand name</rdfs:label>
        <rdfs:comment>Indicates the brand name of the item (ex. BASF, Scotch)</rdfs:comment>
        <rdfs:subPropertyOf rdf:resource="http://jacobshelby.org/schemas/aps/2014/08/03/apsSchema.rdf#brand"/>
        <rdfs:range rdf:resource="http://jacobshelby.org/schemas/aps/2014/08/03/apsSchema.rdf#BrandName"/>
    </rdf:Property>

    <rdf:Property rdf:ID="carrierName">
        <rdfs:label xml:lang="en">carrier name</rdfs:label>
        <rdfs:comment>Specifies the name of the carrier (ex. Lacquer disc or open reel
            tape)</rdfs:comment>
        <rdfs:range rdf:resource="http://jacobshelby.org/schemas/aps/2014/08/03/apsSchema.rdf#Carrier"/>
        <rdfs:domain rdf:resource="http://jacobshelby.org/schemas/aps/2014/08/03/apsSchema.rdf#Carrier"/>
    </rdf:Property>

    <rdf:Property rdf:ID="cassetteType">
        <rdfs:label xml:lang="en">cassette type</rdfs:label>
        <rdfs:comment>Indicates the play type of the cassette (ex. Type I, Type IV)</rdfs:comment>
        <rdfs:range rdf:resource="http://jacobshelby.org/schemas/aps/2014/08/03/apsSchema.rdf#Cassette"/>
        <rdfs:domain rdf:resource="http://jacobshelby.org/schemas/aps/2014/08/03/apsSchema.rdf#Cassette"/>
    </rdf:Property>

    <rdf:Property rdf:ID="child">
        <rdfs:label xml:lang="en">child</rdfs:label>
        <rdfs:comment>Acts as a wrapper for information about a carrier whose content was copied
            from the carrier being described.</rdfs:comment>
    </rdf:Property>

    <rdf:Property rdf:ID="childID">
        <rdfs:label xml:lang="en">child identifier</rdfs:label>
        <rdfs:comment>Indicates an indentifier for an item whose sound recording was copied from the
            item being described.</rdfs:comment>
        <rdfs:range rdf:resource="http://jacobshelby.org/schemas/aps/2014/08/03/apsSchema.rdf#ChildID"/>
    </rdf:Property>

    <rdf:Property rdf:ID="collectionID">
        <rdfs:label xml:lang="en">collection identifier</rdfs:label>
        <rdfs:comment>Indicates an indentifier for the collection that the item belongs
            to.</rdfs:comment>
    </rdf:Property>

    <rdf:Property rdf:ID="condition">
        <rdfs:label xml:lang="en">condition</rdfs:label>
        <rdfs:comment>Acts as a wrapper for condition information</rdfs:comment>
    </rdf:Property>

    <rdf:Property rdf:ID="conditionStatus">
        <rdfs:label xml:lang="en">condition status</rdfs:label>
        <rdfs:comment>Indicates the severity of the condition (ex. Minor, mild, or
            severe)</rdfs:comment>
        <rdfs:subPropertyOf rdf:resource="http://jacobshelby.org/schemas/aps/2014/08/03/apsSchema.rdf#condition"/>
        <rdfs:range rdf:resource="http://jacobshelby.org/schemas/aps/2014/08/03/apsSchema.rdf#ConditionStatus"/>
    </rdf:Property>

    <rdf:Property rdf:ID="datType">
        <rdfs:label xml:lang="en">digital audio tape (DAT) type</rdfs:label>
        <rdfs:comment>Specifies whether the digital audio tape (DAT) is a standard tape or a digital
            data storage tape</rdfs:comment>
        <rdfs:range rdf:resource="http://jacobshelby.org/schemas/aps/2014/08/03/apsSchema.rdf#DAT"/>
        <rdfs:domain rdf:resource="http://jacobshelby.org/schemas/aps/2014/08/03/apsSchema.rdf#DAT"/>
    </rdf:Property>

    <rdf:Property rdf:ID="discSpeed">
        <rdfs:label xml:lang="en">disc speed</rdfs:label>
        <rdfs:comment>Indicates at what speed, in revolutions per minute (RPM), the sound recording
            was recorded onto a disc carrier</rdfs:comment>
        <rdfs:range rdf:resource="http://jacobshelby.org/schemas/aps/2014/08/03/apsSchema.rdf#DiscSpeed"/>
        <rdfs:domain rdf:resource="http://jacobshelby.org/schemas/aps/2014/08/03/apsSchema.rdf#Disc"/>
    </rdf:Property>

    <rdf:Property rdf:ID="generation">
        <rdfs:label xml:lang="en">generation</rdfs:label>
        <rdfs:comment>Indicates the duplication level of a copied carrier. For example, if the
            recording on a carrier was directly transferred from the original carrier, the copy
            would be a first generation copy (ex. 1st, 2nd)</rdfs:comment>
        <rdfs:range rdf:resource="http://jacobshelby.org/schemas/aps/2014/08/03/apsSchema.rdf#OrdinalNumber"/>
    </rdf:Property>

    <rdfs:Property rdf:ID="hasCarrier">
        <rdfs:label xml:lang="en">has carrier</rdfs:label>
        <rdfs:comment>Acts as a wrapper for information about the carrier of the sound
            recording</rdfs:comment>
    </rdfs:Property>

    <rdf:Property rdf:ID="hasCondition">
        <rdfs:label xml:lang="en">has condition</rdfs:label>
        <rdfs:comment>Indicates a condition that the item has (ex. Mold or
            delamination)</rdfs:comment>
        <rdfs:subPropertyOf rdf:resource="http://jacobshelby.org/schemas/aps/2014/08/03/apsSchema.rdf#condition"/>
        <rdfs:range rdf:resource="http://jacobshelby.org/schemas/aps/2014/08/03/apsSchema.rdf#Condition"/>
    </rdf:Property>

    <rdf:Property rdf:ID="id">
        <rdfs:label xml:lang="en">identifier</rdfs:label>
        <rdfs:comment>Indicates an indentifier for the item</rdfs:comment>
        <rdfs:range rdf:resource="http://jacobshelby.org/schemas/aps/2014/08/03/apsSchema.rdf#ID"/>
    </rdf:Property>

    <rdf:Property rdf:ID="manufacturer">
        <rdfs:label xml:lang="en">manufacturer</rdfs:label>
        <rdfs:comment>Indicates the name of the company that manufactures the carrier</rdfs:comment>
        <rdfs:range rdf:resource="http://jacobshelby.org/schemas/aps/2014/08/03/apsSchema.rdf#Manufacturer"/>
        <rdfs:subPropertyOf rdf:resource="http://jacobshelby.org/schemas/aps/2014/08/03/apsSchema.rdf#brand"/>
    </rdf:Property>

    <rdf:Property rdf:ID="material">
        <rdfs:label xml:lang="en">material</rdfs:label>
        <rdfs:comment>Indicates a material used in the creation of the carrier (ex. Aluminum or
            polyester)</rdfs:comment>
        <rdfs:range rdf:resource="http://jacobshelby.org/schemas/aps/2014/08/03/apsSchema.rdf#Material"/>
    </rdf:Property>

    <rdf:Property rdf:ID="modelNumber">
        <rdfs:label xml:lang="en">model number</rdfs:label>
        <rdfs:comment>Indicates the model number of the item (ex. 111 or C-60)</rdfs:comment>
        <rdfs:range rdf:resource="http://jacobshelby.org/schemas/aps/2014/08/03/apsSchema.rdf#ModelNumber"/>
    </rdf:Property>

    <rdf:Property rdf:ID="parent">
        <rdfs:label xml:lang="en">parent</rdfs:label>
        <rdfs:comment>Acts as a wrapper for information about a carrier whose content was copied to
            the carrier being described</rdfs:comment>
    </rdf:Property>

    <rdf:Property rdf:ID="parentID">
        <rdfs:label xml:lang="en">parent identifier</rdfs:label>
        <rdfs:comment>Indicates an identifier for an item whose sound recording was copied to the
            item being described</rdfs:comment>
        <rdfs:range rdf:resource="http://jacobshelby.org/schemas/aps/2014/08/03/apsSchema.rdf#ParentID"/>
    </rdf:Property>

    <rdf:Property rdf:ID="playTime">
        <rdfs:label xml:lang="en">play time</rdfs:label>
        <rdfs:comment>Indicates the duration from beginning to end of the sound recording.
            Recommended best practices are to use the XML data type for duration</rdfs:comment>
    </rdf:Property>

    <rdf:Property rdf:ID="sampleRate">
        <rdfs:label xml:lang="en">sample rate</rdfs:label>
        <rdfs:comment>Indicates the number of samples per second, measured in kiloHertz (kHz), used
            to record the sound recording (ex. 96 kHz)</rdfs:comment>
    </rdf:Property>

    <rdfs:Property rdf:ID="status">
        <rdfs:label xml:lang="en">status</rdfs:label>
        <rdfs:comment>Indicates whether the carrier is the original carrier of the sound recording
            or if the recording was copied from another carrier. If the carrier is a copy, a
            generation statement is required if known.</rdfs:comment>
    </rdfs:Property>

    <rdfs:Property rdf:ID="tapeSpeed">
        <rdfs:label xml:lang="en">tape speed</rdfs:label>
        <rdfs:comment>Indicates at what speed, in inches per second (IPS), the sound recording was
            recorded on a tape carrier</rdfs:comment>
        <rdfs:range rdf:resource="http://jacobshelby.org/schemas/aps/2014/08/03/apsSchema.rdf#TapeSpeed"/>
        <rdfs:domain rdf:resource="http://jacobshelby.org/schemas/aps/2014/08/03/apsSchema.rdf#Tape"/>
    </rdfs:Property>

    <rdf:Property rdf:ID="thickness">
        <rdfs:label xml:lang="en">thickness</rdfs:label>
        <rdfs:comment>Indicates the thickness, in millimeters or inches, of the carrier. Usually
            used for tape carriers, but can be used for wire carriers when needed (ex. 1.5 mil, 1.0
            mil)</rdfs:comment>
        <rdfs:domain rdf:resource="http://jacobshelby.org/schemas/aps/2014/08/03/apsSchema.rdf#Carrier"/>
    </rdf:Property>

    <rdf:Property rdf:ID="trackConfig">
        <rdfs:label xml:lang="en">track configuration</rdfs:label>
        <rdfs:comment>Indicates the track configuration of a tape carrier (e.g., full track or half
            track mono)</rdfs:comment>
        <rdfs:range rdf:resource="http://jacobshelby.org/schemas/aps/2014/08/03/apsSchema.rdf#TrackConfig"/>
        <rdfs:domain rdf:resource="http://jacobshelby.org/schemas/aps/2014/08/03/apsSchema.rdf#Tape"/>
    </rdf:Property>

    <rdf:Property rdf:ID="wireSpeed">
        <rdfs:label xml:lang="en">wire speed</rdfs:label>
        <rdfs:comment>Indicates at what speed, in inches per second (IPS), the sound recording was
            recorded onto a wire carrier</rdfs:comment>
        <rdfs:range rdf:resource="http://jacobshelby.org/schemas/aps/2014/08/03/apsSchema.rdf#WireSpeed"/>
        <rdfs:domain rdf:resource="http://jacobshelby.org/schemas/aps/2014/08/03/apsSchema.rdf#Wire"/>
    </rdf:Property>

    <rdf:Property rdf:ID="wireType">
        <rdfs:label xml:lang="en">wire type</rdfs:label>
        <rdfs:comment>Specifies whether the wire carrier was made before the outbreak of World War
            II or after. Pre-war wires were unstandardized, so statements about wire thickness,
            material, and speed are recommended when the carrier is pre-war</rdfs:comment>
        <rdfs:range rdf:resource="http://jacobshelby.org/schemas/aps/2014/08/03/apsSchema.rdf#Wire"/>
        <rdfs:domain rdf:resource="http://jacobshelby.org/schemas/aps/2014/08/03/apsSchema.rdf#Wire"/>
    </rdf:Property>

    <rdfs:Class rdf:ID="BrandName">
        <rdfs:label xml:lang="en">Brand Name</rdfs:label>
        <rdfs:comment>The name of the brand of the carrier</rdfs:comment>
    </rdfs:Class>

    <rdfs:Class rdf:ID="Carrier">
        <rdfs:label xml:lang="en">Carrier</rdfs:label>
        <rdfs:comment>The physical object on which a sound recording is recorded onto and house
            in</rdfs:comment>
    </rdfs:Class>

    <aps:Carrier rdf:ID="Disc">
        <rdfs:label xml:lang="en">Disc</rdfs:label>
    </aps:Carrier>

    <aps:Disc rdf:ID="AluminumDisc">
        <rdfs:label xml:lang="en">Aluminum Disc</rdfs:label>
        <rdfs:comment>see chapter 5 of the Facet Formats document</rdfs:comment>
        <rdfs:isDefinedBy
            rdf:resource="http://www.dlib.indiana.edu/projects/sounddirections/facet/facet_formats.pdf"
        />
    </aps:Disc>

    <aps:Disc rdf:ID="CD">
        <rdfs:label xml:lang="en">Compact Disc</rdfs:label>
        <rdfs:comment>There are many different types of Compact Discs. I will eventually add these
            to the schema</rdfs:comment>
        <rdfs:isDefinedBy rdf:resource="http://en.wikipedia.org/wiki/Compact_disc"/>
    </aps:Disc>
    <aps:Disc rdf:ID="LacquerDisc">
        <rdfs:label>Lacquer Disc</rdfs:label>
        <rdfs:isDefinedBy rdf:resource="http://en.wikipedia.org/wiki/Acetate_disc"/>
    </aps:Disc>
    <aps:Disc rdf:ID="LP">
        <rdfs:label xml:lang="en">Long Play record</rdfs:label>
        <rdfs:isDefinedBy rdf:resource="http://en.wikipedia.org/wiki/LP_record"/>
    </aps:Disc>
    <aps:Disc rdf:ID="ShellacDisc">
        <rdfs:label xml:lang="en">Shellac Disc</rdfs:label>
        <rdfs:comment>The shellac disc is most commonly referred to as 78s (78 revolutions per
            minute). These are made with a shellac material, which makes them rather
            brittle.</rdfs:comment>
    </aps:Disc>

    <aps:Carrier rdf:ID="Tape">
        <rdfs:label xml:lang="en">Tape</rdfs:label>
    </aps:Carrier>
    <aps:Tape rdf:ID="Cassette">
        <rdfs:label xml:lang="en">Cassette tape</rdfs:label>
        <rdfs:isDefinedBy rdf:resource="http://en.wikipedia.org/wiki/Cassette_tape"/>
    </aps:Tape>
    <aps:Cassette rdf:ID="TypeI">
        <rdfs:label xml:lang="en">Type I</rdfs:label>
        <rdfs:isDefinedBy
            rdf:resource="http://en.wikipedia.org/wiki/Compact_Cassette#Cassette_types"/>
    </aps:Cassette>
    <aps:Cassette rdf:ID="TypeII">
        <rdfs:label xml:lang="en">Type II</rdfs:label>
        <rdfs:isDefinedBy
            rdf:resource="http://en.wikipedia.org/wiki/Compact_Cassette#Cassette_types"/>
    </aps:Cassette>
    <aps:Cassette rdf:ID="TypeIII">
        <rdfs:label xml:lang="en">Type III</rdfs:label>
        <rdfs:isDefinedBy
            rdf:resource="http://en.wikipedia.org/wiki/Compact_Cassette#Cassette_types"/>
    </aps:Cassette>
    <aps:Cassette rdf:ID="TypeIV">
        <rdfs:label xml:lang="en">Type IV</rdfs:label>
        <rdfs:isDefinedBy
            rdf:resource="http://en.wikipedia.org/wiki/Compact_Cassette#Cassette_types"/>
    </aps:Cassette>

    <aps:Tape rdf:ID="DAT">
        <rdfs:label xml:lang="en">Digital Audio Tape</rdfs:label>
        <rdfs:comment>see chapter 4 of the Facet Formats document</rdfs:comment>
        <rdfs:isDefinedBy
            rdf:resource="http://www.dlib.indiana.edu/projects/sounddirections/facet/facet_formats.pdf"
        />
    </aps:Tape>
    <aps:DAT rdf:ID="DDS">
        <rdfs:label xml:lang="en">
            <rdf:Alt>
                <rdf:li>Digital Data Storage</rdf:li>
                <rdf:li>DDS</rdf:li>
                <rdf:li>Data Cartridge</rdf:li>
                <rdf:li>Data Tape</rdf:li>
                <rdf:li>Data-Grade Tape</rdf:li>
            </rdf:Alt>
        </rdfs:label>
        <rdfs:isDefinedBy rdf:resource="http://en.wikipedia.org/wiki/Digital_Data_Storage"/>
        <rdfs:comment>The casing on a DDS DAT tape will have one of the labels listed under this
            class.</rdfs:comment>
    </aps:DAT>

    <aps:DAT rdf:ID="Standard">
        <rdfs:label xml:lang="en">Audio-Grade Tape</rdfs:label>
        <rdfs:comment> Audio-grade DAT tapes are the most standard and safest type of DAT tape. If
            the casing of the tape does not indicate that it is a DDS tape, then it will most likely
            be an audio-grade tape. </rdfs:comment>
    </aps:DAT>

    <aps:Tape rdf:ID="OpenReelTape">
        <rdfs:label>Open Reel Tape</rdfs:label>
        <rdfs:isDefinedBy
            rdf:resource="http://en.wikipedia.org/wiki/Reel-to-reel_audio_tape_recording"/>
    </aps:Tape>

    <aps:Carrier rdf:ID="Wire">
        <rdfs:label>Wire</rdfs:label>
        <rdfs:isDefinedBy rdf:resource="http://en.wikipedia.org/wiki/Wire_recording"/>
    </aps:Carrier>

    <aps:Wire rdf:ID="PreWar">
        <rdfs:label xml:lang="en">Pre World War II Wire</rdfs:label>
        <rdfs:seeAlso
            rdf:resource="http://www.dlib.indiana.edu/projects/sounddirections/facet/facet_formats.pdf"/>
        <rdfs:comment>The following was taken from the Facet Formats documentation: Wires recorded
            before World War II may be steel, but not stainless steel, and subject to corrosion.
            These early wires are also likely a non-standard size and/or speed. The primary
            manufacturer of pre-World War II wire recorders was Armour, which also licensed its
            technology to General Electric. Note that this category is for Armour brand wires, not
            wires from other manufacturers labeled as conforming to the Armour standard.
        </rdfs:comment>
    </aps:Wire>

    <aps:Wire rdf:ID="PostWar">
        <rdfs:label xml:lang="en">Post World War II Wire</rdfs:label>
        <rdfs:seeAlso
            rdf:resource="http://www.dlib.indiana.edu/projects/sounddirections/facet/facet_formats.pdf"/>
        <rdfs:comment>Post World War II wires were stainless steel and the dimensions of the wires
            were standardized</rdfs:comment>
    </aps:Wire>

    <rdfs:Class rdf:ID="Child">
        <rdfs:label xml:lang="en">Child</rdfs:label>
        <rdfs:comment>A carrier whose content was copied from the carrier being
            described</rdfs:comment>
    </rdfs:Class>

    <rdfs:Class rdf:ID="ChildID">
        <rdfs:label xml:lang="en">Child Identifier</rdfs:label>
        <rdfs:comment>A unique identifier for an item that is a copy of the current
            carrier</rdfs:comment>
        <rdfs:subClassOf rdf:resource="http://jacobshelby.org/schemas/aps/2014/08/03/apsSchema.rdf#ID"/>
    </rdfs:Class>

    <rdfs:Class rdf:ID="Condition">
        <rdfs:label xml:lang="en">Condition</rdfs:label>
        <rdfs:comment>Any chemical or physical deformation or substance that jeopardizes the
            integrity of the item or collection</rdfs:comment>
    </rdfs:Class>

    <rdfs:Class rdf:ID="ConditionStatus">
        <rdfs:label xml:lang="en">Condition Status</rdfs:label>
        <rdfs:comment>The level of severity of a condition</rdfs:comment>
    </rdfs:Class>

    <aps:ConditionStatus rdf:ID="Minor">
        <rdfs:label xml:lang="en">Minor</rdfs:label>
    </aps:ConditionStatus>
    <aps:ConditionStatus rdf:ID="Moderate">
        <rdfs:label xml:lang="en">Moderate</rdfs:label>
    </aps:ConditionStatus>
    <aps:ConditionStatus rdf:ID="Severe">
        <rdfs:label xml:lang="en">Severe</rdfs:label>
    </aps:ConditionStatus>

    <rdfs:Class rdf:ID="Copy">
        <rdfs:label xml:lang="en">Copy</rdfs:label>
        <rdfs:comment>A statement indicating that the carrier contains a sound recording that was
            transferred from another carrier.</rdfs:comment>
    </rdfs:Class>

    <rdfs:Class rdf:ID="DiscSpeed">
        <rdfs:label xml:lang="en">Disc Speed</rdfs:label>
        <rdfs:comment>The speed in revolutions per minute (RPM) of a disc carrier</rdfs:comment>
    </rdfs:Class>

    <rdfs:Class rdf:ID="ID">
        <rdfs:label xml:lang="en">Identifier</rdfs:label>
        <rdfs:comment>A unique identifier for the item</rdfs:comment>
    </rdfs:Class>

    <rdfs:Class rdf:ID="Manufacturer">
        <rdfs:label xml:lang="en">Manufacturer</rdfs:label>
        <rdfs:comment>The name of the company who manufactures the carrier</rdfs:comment>
    </rdfs:Class>

    <rdfs:Class rdf:ID="Material">
        <rdfs:label xml:lang="en">Material</rdfs:label>
        <rdfs:comment>A substance that contributes to the creation of the carrier</rdfs:comment>
    </rdfs:Class>

    <rdfs:Class rdf:ID="ModelNumber">
        <rdfs:label xml:lang="en">Model Number</rdfs:label>
        <rdfs:comment>The number of the model of the carrier</rdfs:comment>
    </rdfs:Class>

    <rdfs:Class rdf:ID="OrdinalNumber">
        <rdfs:label xml:lang="en">Ordinal Number</rdfs:label>
        <rdfs:isDefinedBy
            rdf:resource="http://en.wikipedia.org/wiki/English_numerals#Ordinal_numbers"/>
    </rdfs:Class>

    <rdfs:Class rdf:ID="Original">
        <rdfs:label xml:lang="en">Original</rdfs:label>
        <rdfs:comment>A statement indicating that the carrier is the initial carrier on which a
            sound recording was recorded on.</rdfs:comment>
    </rdfs:Class>

    <rdfs:Class rdf:ID="Parent">
        <rdfs:label xml:lang="en">Parent</rdfs:label>
        <rdfs:comment>A carrier whose content was copied to the carrier being
            described</rdfs:comment>
    </rdfs:Class>

    <rdfs:Class rdf:ID="ParentID">
        <rdfs:label xml:lang="en">Parent Identifier</rdfs:label>
        <rdfs:comment>A unique identifier for a carrier in which the current carrier was copied
            from</rdfs:comment>
        <rdfs:subClassOf rdf:resource="http://jacobshelby.org/schemas/aps/2014/08/03/apsSchema.rdf#ID"/>
    </rdfs:Class>

    <rdfs:Class rdf:ID="TapeSpeed">
        <rdfs:label xml:lang="en">Tape Speed</rdfs:label>
        <rdfs:comment>The speed in inches per second (IPS) of a tape carrier</rdfs:comment>
    </rdfs:Class>

    <rdfs:Class rdf:ID="TrackConfig">
        <rdfs:label xml:lang="en">Track Configuration</rdfs:label>
        <rdfs:comment>The track configuration of a tape carrier. See section 2.2.5 of the Facet
            Formats document.</rdfs:comment>
        <rdfs:seeAlso
            rdf:resource="http://www.dlib.indiana.edu/projects/sounddirections/facet/facet_formats.pdf"
        />
    </rdfs:Class>

    <aps:TrackConfig rdf:ID="FullTrack">
        <rdfs:label xml:lang="en">Full Track</rdfs:label>
    </aps:TrackConfig>
    <aps:TrackConfig rdf:ID="HalfTrackMono">
        <rdfs:label>Halftrack Mono</rdfs:label>
    </aps:TrackConfig>
    <aps:TrackConfig rdf:ID="HalfTrackStereo">
        <rdfs:label>Halftrack Stereo</rdfs:label>
    </aps:TrackConfig>
    <aps:TrackConfig rdf:ID="QuarterTrackMono">
        <rdfs:label>Quartertrack Mono</rdfs:label>
    </aps:TrackConfig>
    <aps:TrackConfig rdf:ID="QuarterTrackStereo">
        <rdfs:label>Quartertrack Stereo</rdfs:label>
    </aps:TrackConfig>

    <rdfs:Class rdf:ID="WireSpeed">
        <rdfs:label xml:lang="en">Wire Speed</rdfs:label>
        <rdfs:comment>The speed in inches per second (IPS) of a wire carrier</rdfs:comment>
    </rdfs:Class>

</rdf:RDF>
